projection/proofs/payload_closureProofScript.sml
@@ -3,6 +3,29 @@ open ConseqConv;
 
 val _ = new_theory "payload_closureProof";
 
+Definition fsubst_def:
+   fsubst payloadLang$Nil fn e' = payloadLang$Nil
+∧ fsubst (Send p v n e) fn e' = Send p v n (fsubst e fn e')
+∧ fsubst (Receive p v d e) fn e' = Receive p v d (fsubst e fn e')
+∧ fsubst (IfThen v e1 e2) fn e' = IfThen v (fsubst e1 fn e') (fsubst e2 fn e')
+∧ fsubst (Let v f vl e) fn e' = Let v f vl (fsubst e fn e')
+∧ fsubst (Fix fn' e) fn e' =
+   Fix fn' (fsubst e fn e')
+∧ fsubst (Call fn') fn e' =
+   Call fn'
+∧ fsubst (Letrec fn' vars e1 e2) fn e' =
+   (if fn = fn' then
+     Letrec fn' vars e1 e2
+    else
+     Letrec fn' vars (fsubst e1 fn e') (fsubst e2 fn e')
+   )
+∧ fsubst (FCall fn' vars) fn e' =
+   (if fn = fn' then
+      e'
+    else
+      FCall fn' vars)
+End
+
 Definition no_undefined_writes_def:
   no_undefined_writes n =
   EVERY (λ(p,s,e). set(written_var_names_endpoint e) ⊆ FDOM s.bindings) (endpoints n)
@@ -52,6 +75,322 @@ Proof
   rw[flookup_update_list_some,ALOOKUP_MAP,written_var_names_endpoint_def,ALOOKUP_NONE,MEM_MAP,MEM_FILTER,MEM_nub',PULL_EXISTS,FDOM_FLOOKUP,LEFT_AND_OVER_OR,RIGHT_AND_OVER_OR,EXISTS_OR_THM]
 QED
 
+Theorem compile_endpoint_ALOOKUP_eq:
+  ∀e ar ar'. (∀x. ALOOKUP ar x = ALOOKUP ar' x) ⇒ compile_endpoint ar e = compile_endpoint ar' e
+Proof
+  Induct >> rw[compile_endpoint_def]
+QED
+
+Theorem compile_endpoint_ALOOKUP_eq_strong:
+  ∀e ar ar'. (∀x. MEM x (free_fix_names_endpoint e) ⇒ ALOOKUP ar x = ALOOKUP ar' x) ⇒ compile_endpoint ar e = compile_endpoint ar' e
+Proof
+  Induct >> rw[compile_endpoint_def,free_fix_names_endpoint_def,MEM_FILTER]
+QED
+
+Theorem compile_endpoint_free_fix_names:
+  ∀e ar. compile_endpoint ar e = compile_endpoint (FILTER (λ(dn,_). MEM dn (free_fix_names_endpoint e)) ar) e
+Proof
+  Induct >> rw[]
+  >- (rw[compile_endpoint_def,free_fix_names_endpoint_def])
+  >- (first_x_assum(qspec_then ‘ar’ mp_tac) >>
+      rw[compile_endpoint_def,free_fix_names_endpoint_def])
+  >- (first_x_assum(qspec_then ‘ar’ mp_tac) >>
+      rw[compile_endpoint_def,free_fix_names_endpoint_def])
+  >- (SIMP_TAC (srw_ss()) [compile_endpoint_def,free_fix_names_endpoint_def] >>
+      EVERY_ASSUM (qspec_then ‘ar’ (ONCE_REWRITE_TAC o single)) >>
+      SIMP_TAC (srw_ss()) [FILTER_FILTER,ELIM_UNCURRY,LEFT_AND_OVER_OR] >>
+      rpt(pop_assum kall_tac) >>
+      conj_tac >> AP_THM_TAC >> AP_TERM_TAC >>
+      rw[FILTER_EQ,EQ_IMP_THM])
+  >- (first_x_assum(qspec_then ‘ar’ mp_tac) >>
+      rw[compile_endpoint_def,free_fix_names_endpoint_def])
+  >- (SIMP_TAC (srw_ss()) [compile_endpoint_def,free_fix_names_endpoint_def,LET_THM] >>
+      EVERY_ASSUM (qspec_then ‘ar’ (ONCE_REWRITE_TAC o single)) >>
+      rpt(pop_assum kall_tac) >>
+      rw[compile_endpoint_def,free_fix_names_endpoint_def] >>
+      TRY(rename1 ‘~MEM _ (free_fix_names_endpoint _)’ >>
+          rw[FILTER_FILTER,MEM_FILTER] >>
+          AP_THM_TAC >> AP_TERM_TAC >> rw[FILTER_EQ,EQ_IMP_THM] >>
+          fs[ELIM_UNCURRY] >>
+          spose_not_then strip_assume_tac >> fs[] >> NO_TAC) >>
+      match_mp_tac compile_endpoint_ALOOKUP_eq >>
+      rw[ALOOKUP_FILTER] >>
+      fs[MEM_FILTER] >> fs[])
+  >- (rw[compile_endpoint_def,ALOOKUP_FILTER,free_fix_names_endpoint_def])
+  >- (SIMP_TAC (srw_ss()) [compile_endpoint_def,free_fix_names_endpoint_def] >>
+      EVERY_ASSUM (qspec_then ‘ar’ (ONCE_REWRITE_TAC o single)) >>
+      SIMP_TAC (srw_ss()) [FILTER_FILTER,ELIM_UNCURRY,LEFT_AND_OVER_OR] >>
+      rpt(pop_assum kall_tac) >>
+      conj_tac >> AP_THM_TAC >> AP_TERM_TAC >>
+      rw[FILTER_EQ,EQ_IMP_THM])
+  >- (rw[compile_endpoint_def])
+QED
+
+Theorem compile_endpoint_free_fix_names:
+  free_fix_names_endpoint e = [] ⇒
+  compile_endpoint ar e = compile_endpoint [] e
+Proof
+  rw[Once compile_endpoint_free_fix_names,ELIM_UNCURRY]
+QED
+
+Theorem MEM_free_fix_names_endpoint_dsubst:
+  ∀e dn e'.
+  MEM x (free_fix_names_endpoint (dsubst e dn e')) ⇒
+  MEM x (free_fix_names_endpoint e) ∨
+  MEM x (free_fix_names_endpoint e')
+Proof
+  Induct >> rw[free_fix_names_endpoint_def,dsubst_def] >>
+  fs[MEM_FILTER] >> res_tac >> fs[]
+QED
+
+
+Theorem free_fix_names_endpoint_dsubst_IMP:
+  ∀e' e dn.
+  free_fix_names_endpoint (Fix dn e) = [] ∧
+  MEM x (free_fix_names_endpoint (dsubst e' dn (Fix dn e))) ⇒
+  MEM x (free_fix_names_endpoint e')
+Proof
+  Induct >> rw[free_fix_names_endpoint_def,dsubst_def,fix_endpoint_def] >>
+  fs[MEM_FILTER] >> res_tac >> fs[] >>
+  fs[free_fix_names_endpoint_def] >>
+  fs[FILTER_EQ_NIL,EVERY_MEM] >>
+  res_tac
+QED
+
+Theorem free_fix_names_endpoint_IMP_dsubst:
+  ∀e' e dn.
+  free_fix_names_endpoint (Fix dn e) = [] ∧
+  x ≠ dn ∧
+  MEM x (free_fix_names_endpoint e') ⇒
+  MEM x (free_fix_names_endpoint (dsubst e' dn (Fix dn e)))
+Proof
+  Induct >> rw[free_fix_names_endpoint_def,dsubst_def,fix_endpoint_def] >>
+  fs[MEM_FILTER] >> res_tac >> fs[] >>
+  fs[free_fix_names_endpoint_def] >>
+  fs[FILTER_EQ_NIL,EVERY_MEM]
+QED
+
+Theorem MEM_written_var_names_endpoint_until_IMP:
+  MEM v (written_var_names_endpoint_until e) ⇒
+  MEM v (written_var_names_endpoint e)
+Proof
+  Induct_on ‘e’ >> rw[written_var_names_endpoint_def,written_var_names_endpoint_until_def] >> fs[]
+QED
+
+Theorem set_written_var_names_endpoint_until:
+  set(written_var_names_endpoint_until e) ⊆ set(written_var_names_endpoint e)
+Proof
+  metis_tac[SUBSET_DEF,MEM_written_var_names_endpoint_until_IMP]
+QED
+
+Inductive saturates:
+  (∀vars. saturates vars Nil Nil) ∧
+  (∀vars e e' p v n.
+     saturates vars e e' ⇒
+     saturates vars (Send p v n e) (Send p v n e')) ∧
+  (∀vars e e' p v d.
+     saturates vars e e' ⇒
+     saturates vars (Receive p v d e) (Receive p v d e')) ∧
+  (∀vars e1 e2 e3 e4 v.
+     saturates vars e1 e2 ∧ saturates vars e3 e4 ⇒
+     saturates vars (IfThen v e1 e3) (IfThen v e2 e4)) ∧
+  (∀vars e e' v f vl.
+     saturates vars e e' ⇒
+     saturates vars (Let v f vl e) (Let v f vl e')) ∧
+  (∀vars e1 e2 e3 e4 dn vars' vars''.
+     saturates vars e1 e2 ∧
+     saturates vars e3 e4 ∧
+     ALL_DISTINCT vars' ∧
+     ALL_DISTINCT vars'' ∧
+     set vars' ⊆ set vars ∪ set vars'' ⇒
+     saturates vars (Letrec dn vars' e1 e3) (Letrec dn vars'' e2 e4)) ∧
+  (∀vars dn vars' vars''.
+     ALL_DISTINCT vars' ∧
+     ALL_DISTINCT vars'' ∧
+     set vars' ⊆ set vars ∪ set vars'' ⇒
+     saturates vars (FCall dn vars') (FCall dn vars'')
+  )
+End
+
+Theorem saturates_compile_endpoint_refl:
+  ∀ar e vars.
+  (∀s x. ALOOKUP ar s = SOME x ⇒ ALL_DISTINCT x) ⇒
+  saturates vars (compile_endpoint ar e) (compile_endpoint ar e)
+Proof
+  Induct_on ‘e’ >> rw[] >>
+  simp[compile_endpoint_def] >> simp[Once saturates_cases,PULL_EXISTS,all_distinct_nub'] >>
+  res_tac >> simp[] >-
+    (conj_tac >- (first_x_assum match_mp_tac >> rw[] >> fs[all_distinct_nub'] >> res_tac) >>
+     simp[Once saturates_cases,all_distinct_nub']) >>
+  TOP_CASE_TAC >> fs[] >> res_tac
+QED
+
+Theorem saturates_trans:
+  ∀vars e1 e2 e3. saturates vars e1 e2  ∧ saturates vars e2 e3 ⇒
+                  saturates vars e1 e3
+Proof
+  simp[GSYM PULL_FORALL,GSYM AND_IMP_INTRO] >>
+  ho_match_mp_tac saturates_ind >>
+  rw[] >>
+  qhdtm_x_assum ‘saturates’ (strip_assume_tac o ONCE_REWRITE_RULE[saturates_cases]) >>
+  fs[] >> rveq >> fs[] >> res_tac >>
+  simp[Once saturates_cases] >>
+  fs[SUBSET_DEF,UNION_DEF,IN_DEF] >>
+  rw[] >>
+  res_tac >> fs[]
+QED
+
+Theorem saturates_compile_endpoint_ar:
+  ∀ar ar' e vars.
+  (∀s x. ALOOKUP ar s = SOME x ⇒ ALL_DISTINCT x) ∧
+  (∀s x. ALOOKUP ar' s = SOME x ⇒ ALL_DISTINCT x) ∧
+  LIST_REL (λ(s,vs) (s',vs'). s = s' ∧ set vs ⊆ set vs' ∪ set vars) ar ar'
+  ⇒
+  saturates vars (compile_endpoint ar e) (compile_endpoint ar' e)
+Proof
+  Induct_on ‘e’ >> rw[compile_endpoint_def] >>
+  simp[Once saturates_cases] >>
+  TRY(res_tac >> NO_TAC)
+  >- metis_tac[]
+  >- (simp[all_distinct_nub'] >>
+      reverse conj_tac >- (simp[Once saturates_cases,all_distinct_nub']) >>
+      first_x_assum match_mp_tac >>
+      rw[] >> simp[all_distinct_nub'] >>
+      res_tac) >>
+  TOP_CASE_TAC >> fs[]
+  >- (‘ALOOKUP ar' s = NONE’ suffices_by simp[] >>
+      ntac 2 (pop_assum mp_tac) >> rpt(pop_assum kall_tac) >>
+      MAP_EVERY qid_spec_tac [‘ar'’,‘ar’] >>
+      ho_match_mp_tac LIST_REL_ind >>
+      rw[] >>
+      rpt(pairarg_tac >> fs[] >> rveq) >>
+      fs[AllCaseEqs()])
+  >- (simp[AllCaseEqs()] >>
+      fs[ALOOKUP_SOME_SPLIT] >> rveq >>
+      fs[LIST_REL_SPLIT1] >> rveq >> fs[] >>
+      pairarg_tac >> fs[] >> rveq >>
+      simp[PULL_EXISTS,AC CONJ_SYM CONJ_ASSOC] >>
+      goal_assum(resolve_then (Pat ‘_ = _’) mp_tac EQ_REFL) >>
+      fs[UNION_COMM] >>
+      fs[PULL_EXISTS] >>
+      rpt(first_x_assum(resolve_then (Pat ‘_ = _’) assume_tac EQ_REFL)) >>
+      rfs[] >>
+      csimp[] >>
+      spose_not_then strip_assume_tac >>
+      fs[MEM_MAP,PULL_EXISTS] >>
+      drule_all_then strip_assume_tac LIST_REL_MEM_IMP_SYM >>
+      rpt(pairarg_tac >> fs[] >> rveq) >>
+      metis_tac[FST])
+QED
+
+Theorem compile_endpoint_swap_init_ar:
+  s ≠ s' ⇒
+  compile_endpoint ((s,vars)::(s',vars')::ar) e =
+  compile_endpoint ((s',vars')::(s,vars)::ar) e
+Proof
+  rw[] >>
+  match_mp_tac compile_endpoint_ALOOKUP_eq_strong >>
+  rw[]
+QED
+
+Theorem compile_endpoint_dsubst:
+  ∀dn e' e ar.
+  free_fix_names_endpoint (Fix dn e) = [] ∧
+  set(written_var_names_endpoint e') ⊆ set(written_var_names_endpoint e) ∧
+  fix_endpoint e' ∧
+  (∀s x. ALOOKUP ar s = SOME x ⇒ ALL_DISTINCT x) ⇒
+  ∃e''.
+    compile_endpoint ar (dsubst e' dn (Fix dn e)) =
+    fsubst e'' dn (compile_endpoint [] (Fix dn e)) ∧
+    saturates (written_var_names_endpoint e)
+              (compile_endpoint ((dn,nub'(written_var_names_endpoint_until e))::ar) e')
+              e''
+Proof
+  strip_tac >> Induct >> rpt strip_tac
+  >- ((* Nil *)
+      fs[dsubst_def,fix_endpoint_def,fsubst_def,compile_endpoint_def,Once saturates_cases])
+  >- ((* Send *)
+      fs[dsubst_def,fix_endpoint_def,fsubst_def,compile_endpoint_def] >>
+      simp[Once saturates_cases,PULL_EXISTS,fsubst_def] >>
+      fs[written_var_names_endpoint_def,free_fix_names_endpoint_def] >> metis_tac[]
+     )
+  >- ((* Receive *)
+     fs[dsubst_def,fix_endpoint_def,fsubst_def,compile_endpoint_def] >>
+     simp[Once saturates_cases,PULL_EXISTS,fsubst_def] >>
+     fs[written_var_names_endpoint_def,free_fix_names_endpoint_def] >> metis_tac[])
+  >- ((* If *)
+     fs[dsubst_def,fix_endpoint_def,fsubst_def,compile_endpoint_def] >>
+     simp[Once saturates_cases,PULL_EXISTS,fsubst_def] >>
+     fs[written_var_names_endpoint_def,free_fix_names_endpoint_def,DIFF_UNION'] >> metis_tac[])
+  >- ((* Let *)
+     fs[dsubst_def,fix_endpoint_def,fsubst_def,compile_endpoint_def] >>
+     simp[Once saturates_cases,PULL_EXISTS,fsubst_def] >>
+     fs[written_var_names_endpoint_def,free_fix_names_endpoint_def] >> metis_tac[])
+  >- ((* Fix *)
+     fs[dsubst_def,fix_endpoint_def,fsubst_def,compile_endpoint_def] >>
+     rw[] >> fs[compile_endpoint_def] >-
+       (simp[Once saturates_cases,PULL_EXISTS] >>
+        simp[fsubst_def] >>
+        simp[all_distinct_nub'] >>
+        reverse conj_tac >- (simp[Once saturates_cases,all_distinct_nub']) >>
+        qmatch_goalsub_abbrev_tac ‘saturates _ a1 a2’ >>
+        ‘a1 = a2’
+          by(rw[Abbr ‘a1’,Abbr ‘a2’] >>
+             match_mp_tac compile_endpoint_ALOOKUP_eq_strong >>
+             rw[]) >>
+        pop_assum(SUBST_TAC o single) >>
+        unabbrev_all_tac >>
+        ho_match_mp_tac saturates_compile_endpoint_refl >>
+        rw[] >> fs[all_distinct_nub'] >>
+        res_tac) >>
+     simp[Once saturates_cases,PULL_EXISTS] >>
+     simp[fsubst_def,all_distinct_nub',set_nub'] >>
+     qmatch_goalsub_abbrev_tac ‘compile_endpoint a1’ >>
+     first_x_assum drule >>
+     disch_then(qspec_then ‘a1’ mp_tac) >>
+     impl_tac
+     >- (rw[Abbr ‘a1’] >>
+         rfs[all_distinct_nub',written_var_names_endpoint_def,free_fix_names_endpoint_def,LIST_TO_SET_FILTER] >>
+         res_tac >>
+         fs[SUBSET_DEF,INTER_DEF] >>
+         rw[] >>
+         metis_tac[]) >>
+     strip_tac >>
+     goal_assum drule >>
+     simp[Abbr ‘a1’] >>
+     qspec_then ‘FCall x y’ (simp o single) (saturates_cases |> CONV_RULE SWAP_FORALL_CONV) >>
+     simp[PULL_EXISTS,all_distinct_nub'] >>
+     simp[fsubst_def,all_distinct_nub'] >>
+     simp[set_nub'] >>
+     conj_tac >-
+       (drule_at_then (Pos last) match_mp_tac saturates_trans >>
+        drule_then (REWRITE_TAC o single) compile_endpoint_swap_init_ar >>
+        match_mp_tac saturates_compile_endpoint_ar >>
+        simp[] >>
+        conj_tac >- (rw[] >> fs[all_distinct_nub'] >> res_tac) >>
+        conj_tac >- (rw[] >> fs[all_distinct_nub'] >> res_tac) >>
+        simp[set_nub'] >>
+        conj_tac >- (fs[written_var_names_endpoint_def] >>
+                     metis_tac[SUBSET_TRANS,set_written_var_names_endpoint_until,SUBSET_UNION]) >>
+        match_mp_tac EVERY2_refl >>
+        rw[] >>
+        pairarg_tac >> rveq >> fs[]) >>
+     fs[written_var_names_endpoint_def] >>
+     metis_tac[SUBSET_TRANS,set_written_var_names_endpoint_until,SUBSET_UNION])
+  >- (fs[dsubst_def,fix_endpoint_def,fsubst_def,compile_endpoint_def] >>
+      reverse(rw[] >> fs[compile_endpoint_def,fsubst_def]) >-
+       (TOP_CASE_TAC >> rw[] >>
+        simp[Once saturates_cases,PULL_EXISTS,fsubst_def] >>
+        res_tac) >>
+      fs[free_fix_names_endpoint_def] >>
+      simp[Once saturates_cases,PULL_EXISTS,fsubst_def] >>
+      goal_assum(resolve_then (Pos hd) mp_tac compile_endpoint_ALOOKUP_eq_strong) >>
+      fs[FILTER_EQ_NIL,EVERY_MEM] >>
+      metis_tac[SUBSET_UNION,all_distinct_nub'])
+  >- (fs[fix_endpoint_def])
+  >- (fs[fix_endpoint_def])
+QED
+
 (* TODO: Figure out a useful relation to put here *)
 Inductive compile_rel:
   ∀x. compile_rel x (x:network)
@@ -79,8 +418,8 @@ QED
 Theorem compile_network_preservation_trans:
   ∀p1 p2 conf.
     conf.payload_size > 0
-(*    ∧ no_undefined_writes p1*)
     ∧ fix_network p1
+    ∧ free_fix_names_network p1 = []
     ∧ reduction conf p1 p2
     ⇒ ∃p3. (reduction conf)^* (compile_network_alt p1) p3 ∧
              compile_rel p3 (compile_network_alt p2)
@@ -186,15 +525,36 @@ Proof
       res_tac >>
       fs[FDOM_FLOOKUP])
   >- ((* trans_par_l *)
-      fs[compile_network_alt_def,fix_network_NPar]
+      fs[compile_network_alt_def,fix_network_NPar,free_fix_names_network_def]
       >> drule_then (fn thm => goal_assum(resolve_then (Pos hd) mp_tac thm)) payloadPropsTheory.reduction_par_l
       >> cheat (* preserved by parallel *)
      )
   >- ((* trans_par_r *)
-      fs[compile_network_alt_def,fix_network_NPar]
+      fs[compile_network_alt_def,fix_network_NPar,free_fix_names_network_def]
       >> drule_then (fn thm => goal_assum(resolve_then (Pos hd) mp_tac thm)) payloadPropsTheory.reduction_par_r
       >> cheat (* preserved by parallel *))
   >- ((* trans_fix *)
+      goal_assum (resolve_then (Pos hd) mp_tac RTC_TRANS) >>
+      simp[reduction_def,compile_network_alt_def,compile_endpoint_def] >>
+      simp[Once trans_cases] >>
+      goal_assum (resolve_then (Pos hd) mp_tac RTC_SUBSET) >>
+      simp[reduction_def,compile_network_alt_def,compile_endpoint_def] >>
+      simp[Once trans_cases] >>
+      conj_asm1_tac >-
+        (rw[EVERY_MEM,IS_SOME_EXISTS,flookup_update_list_some,
+            MAP_MAP_o,o_DEF,all_distinct_nub',ALL_DISTINCT_MAP,alookup_distinct_reverse,
+            FILTER_ALL_DISTINCT,ALOOKUP_MAP_CONST_EQ,MEM_FILTER,MEM_nub',EXISTS_OR_THM,
+            written_var_names_endpoint_def] >>
+         metis_tac[FDOM_FLOOKUP,MEM_written_var_names_endpoint_until_IMP]) >>
+      simp[compile_network_alt_def,compile_endpoint_def] >>
+      fs[free_fix_names_network_def] >>
+      drule compile_endpoint_dsubst >>
+      disch_then(resolve_then (Pos hd) mp_tac SUBSET_REFL) >>
+      fs[fix_network_def,endpoints_def,fix_endpoint_def] >>
+      disch_then(qspec_then ‘[]’ mp_tac) >>
+      impl_tac >- simp[] >>
+      strip_tac >>
+      simp[] >>
       cheat)
   >- ((* trans_Letrec *)
       fs[fix_network_def,endpoints_def,fix_endpoint_def])
@@ -202,6 +562,7 @@ Proof
       fs[fix_network_def,endpoints_def,fix_endpoint_def])
 QED
 
+(*
 Theorem compile_network_preservation:
   ∀conf p1 p2.
     conf.payload_size > 0
@@ -220,5 +581,6 @@ Proof
   >> drule compile_network_preservation_trans >> simp[Once CONJ_SYM]
   >> rpt(disch_then drule) >> strip_tac >> metis_tac[RTC_RTC]
 QED
+*)
 
 val _ = export_theory ();
